Towards CoGT and CoLT

theories/Global.v
@@ -15,14 +15,11 @@ Section Syntax.
   (**
    * Global Types
    *)
-  Inductive g_ty A :=
+  Inductive g_ty :=
   | g_end
   | g_var (v : rvar)
-  | g_rec (G : g_ty A)
-  | g_msg (a : A) (p : role) (q : role) (Ks : seq (lbl * (mty * g_ty A))).
-
-  Arguments g_end [_].
-  Arguments g_var [_].
+  | g_rec (G : g_ty)
+  | g_msg (p : role) (q : role) (Ks : seq (lbl * (mty * g_ty))).
 
   Open Scope mpst_scope.
 
@@ -30,20 +27,20 @@ Section Syntax.
   Notation gfv a := (g_var (fv a)).
   Notation gbv n := (g_var (bv n)).
 
-  Fixpoint depth_gty A (a : g_ty A) :=
+  Fixpoint depth_gty (a : g_ty) :=
     match a with
     | g_end
     | g_var _ => 0
     | g_rec G => (depth_gty G).+1
-    | g_msg _ _ _ K => (maximum (map (fun x=> depth_gty x.cnt) K)).+1
+    | g_msg _ _ K => (maximum (map (fun x=> depth_gty x.cnt) K)).+1
     end.
 
-  Fixpoint participants A (G : g_ty A) :=
+  Fixpoint participants (G : g_ty) :=
     match G with
     | g_end
     | g_var _ => [::]
     | g_rec G => participants G
-    | g_msg _ p q Ks => p::q::flatten [seq participants K.cnt | K <- Ks]
+    | g_msg p q Ks => p::q::flatten [seq participants K.cnt | K <- Ks]
     end.
 
   Fixpoint flat_set (A : choiceType) (L : seq {fset A}) :=
@@ -52,39 +49,38 @@ Section Syntax.
     | x::xs => x `|` flat_set xs
     end%fset.
 
-  Fixpoint parts_set A (G : g_ty A) :=
+  Fixpoint parts_set (G : g_ty) :=
     match G with
     | g_end
     | g_var _ => fset0
     | g_rec G => parts_set G
-    | g_msg _ p q Ks => p |` (q |` flat_set [seq parts_set K.cnt | K <- Ks])
+    | g_msg p q Ks => p |` (q |` flat_set [seq parts_set K.cnt | K <- Ks])
     end%fset.
 
   Lemma gty_ind1 :
-    forall A (P : g_ty A -> Prop),
+    forall (P : g_ty -> Prop),
       P g_end ->
       (forall v, P (g_var v)) ->
       (forall G, P G -> P (g_rec G)) ->
-      (forall m p q Ks, (forall K, member K Ks -> P K.cnt) ->
-                        P (g_msg m p q Ks)) ->
-      forall g : g_ty A, P g.
+      (forall p q Ks, (forall K, member K Ks -> P K.cnt) ->
+                        P (g_msg p q Ks)) ->
+      forall g : g_ty, P g.
   Proof.
-    move=> A P P_end P_var P_rec P_msg; fix Ih 1; case.
+    move=> P P_end P_var P_rec P_msg; fix Ih 1; case.
     + by apply: P_end.
     + by apply: P_var.
     + by move=>G; apply: P_rec.
-    + move=>m p q Ks; apply: P_msg.
+    + move=>p q Ks; apply: P_msg.
       by apply/forall_member; elim: Ks.
   Qed.
 
-  Fixpoint eq_g_ty (A : eqType) (a b : g_ty A) :=
+  Fixpoint eq_g_ty (a b : g_ty) :=
     match a, b with
     | g_end, g_end => true
     | g_var v1, g_var v2 => v1 == v2
     | g_rec G1, g_rec G2 => eq_g_ty G1 G2
-    | g_msg m1 p1 q1 Ks1, g_msg m2 p2 q2 Ks2 =>
-      (m1 == m2)
-        && (p1 == p2)
+    | g_msg p1 q1 Ks1, g_msg p2 q2 Ks2 =>
+        (p1 == p2)
         && (q1 == q2)
         && (fix eqL Ks1 Ks2 :=
               match Ks1, Ks2 with
@@ -98,25 +94,25 @@ Section Syntax.
     | _, _ => false
     end.
 
-  Definition eq_alt (A : eqType) (l r : lbl * (mty * g_ty A)) :=
+  Definition eq_alt (l r : lbl * (mty * g_ty)) :=
     (l.lbl == r.lbl) && (l.mty == r.mty) && eq_g_ty l.cnt r.cnt.
 
-  Lemma eqgty_all (A : eqType) m1 p1 q1 (Ks1 : seq (lbl * (mty * g_ty A))) m2 p2 q2 Ks2 :
-    eq_g_ty (g_msg m1 p1 q1 Ks1) (g_msg m2 p2 q2 Ks2) =
-    (m1 == m2) && (p1 == p2) && (q1 == q2) && all2 (eq_alt (A:=A)) Ks1 Ks2.
+  Lemma eqgty_all p1 q1 (Ks1 : seq (lbl * (mty * g_ty))) p2 q2 Ks2 :
+    eq_g_ty (g_msg p1 q1 Ks1) (g_msg p2 q2 Ks2) =
+    (p1 == p2) && (q1 == q2) && all2 eq_alt Ks1 Ks2.
   Proof.
-    rewrite /=; do 3 (case: eqP=>///= _).
+    rewrite /=; do 2 (case: eqP=>///= _).
     by elim: Ks1 Ks2=>[|Ks1 K1 Ih]; case=>[|Ks2 K2]//; rewrite Ih.
   Qed.
 
-  Lemma g_ty_eqP (A: eqType) : Equality.axiom (eq_g_ty (A:=A)).
+  Lemma g_ty_eqP : Equality.axiom eq_g_ty.
   Proof.
     rewrite /Equality.axiom; fix Ih 1 => x y.
-    case x =>[|vl| Gl |ml pl ql Ksl]; case y =>[|vr| Gr |mr pr qr Ksr];
+    case x =>[|vl| Gl |pl ql Ksl]; case y =>[|vr| Gr |pr qr Ksr];
       try (by constructor).
     + by rewrite /eq_g_ty; case: eqP=>[->|H];constructor=>//[[]].
     + by rewrite /=; case: Ih=>[->|H];constructor=>//[[]].
-    + rewrite eqgty_all; do 3 (case: eqP=>[<-|H];[|constructor=>[[]]//] =>/=).
+    + rewrite eqgty_all; do 2 (case: eqP=>[<-|H];[|constructor=>[[]]//] =>/=).
       elim: Ksl Ksr =>[|[ll [tl Gl]] Ksl IhKs].
       - case; try (by constructor).
       - move=>[|[lr [tr Gr] Ksr]/=]; first (by constructor).
@@ -125,10 +121,10 @@ Section Syntax.
         by case: IhKs=>[[]<-|F]; constructor=>//[[F']]; move: F' F=>->.
   Qed.
 
-  Definition g_ty_eqMixin (A : eqType) := EqMixin (g_ty_eqP (A:=A)).
-  Canonical g_ty_eqType (A: eqType) := Eval hnf in EqType (g_ty A) (g_ty_eqMixin A).
+  Definition g_ty_eqMixin := EqMixin g_ty_eqP.
+  Canonical g_ty_eqType := Eval hnf in EqType g_ty g_ty_eqMixin.
 
-  Lemma alt_eqP (A : eqType) : Equality.axiom (eq_alt (A:=A)).
+  Lemma alt_eqP : Equality.axiom eq_alt.
   Proof.
     rewrite /Equality.axiom/eq_alt; move=>[l1  [t1 Ks1]] [l2 [t2 Ks2]]/=.
     do 2 (case: eqP=>[<-|H]; last (by apply: ReflectF => [[/H]])).
@@ -136,54 +132,43 @@ Section Syntax.
   Qed.
 
   Lemma gty_ind2 :
-    forall A (P : g_ty A -> Prop),
+    forall (P : g_ty -> Prop),
       P g_end ->
       (forall v, P (g_var v)) ->
       (forall G, P G -> P (g_rec G)) ->
-      (forall m p q Ks, Forall (fun K => P K.cnt) Ks -> P (g_msg m p q Ks)) ->
-      forall G : g_ty A, P G.
+      (forall p q Ks, Forall (fun K => P K.cnt) Ks -> P (g_msg p q Ks)) ->
+      forall G : g_ty, P G.
   Proof.
-    move=> A P P_end P_var P_rec P_msg; elim/gty_ind1=>//.
-    by move=> m p q Ks /forall_member; apply: P_msg.
+    move=> P P_end P_var P_rec P_msg; elim/gty_ind1=>//.
+    by move=> p q Ks /forall_member; apply: P_msg.
   Qed.
 
-  Fixpoint g_open A (d : nat) (G2 : g_ty A) (G1 : g_ty A) :=
+  Fixpoint g_open (d : nat) (G2 : g_ty) (G1 : g_ty) :=
     match G1 with
     | g_end => G1
-    | g_var v => open (@g_var A) d G2 v
+    | g_var v => open g_var d G2 v
     | g_rec G => g_rec (g_open d.+1 G2 G)
-    | g_msg m p q Ks =>
-      g_msg m p q [seq (K.lbl, (K.mty, g_open d G2 K.cnt)) | K <- Ks]
+    | g_msg p q Ks =>
+      g_msg p q [seq (K.lbl, (K.mty, g_open d G2 K.cnt)) | K <- Ks]
     end.
   Notation "{ k '~>' v } G":= (g_open k v G) (at level 30, right associativity).
   Notation "G '^' v":= (g_open 0 (gfv v) G) (at level 30, right associativity).
 
-  Fixpoint g_close A (v : atom) (d : nat) (G1 : g_ty A) :=
+  Fixpoint g_close (v : atom) (d : nat) (G1 : g_ty) :=
     match G1 with
     | g_end => G1
     | g_var gv => g_var (close v d gv)
     | g_rec G => g_rec (g_close v d.+1 G)
-    | g_msg m p q Ks => g_msg m p q [seq (K.lbl, (K.mty, g_close v d K.cnt)) | K <- Ks]
+    | g_msg p q Ks => g_msg p q [seq (K.lbl, (K.mty, g_close v d K.cnt)) | K <- Ks]
     end.
   Notation "{ k '<~' v } G":= (g_close v k G) (at level 30, right associativity).
 
-  Definition fsetUs (K : choiceType) : seq {fset K} -> {fset K}
-    := foldl fsetU fset0.
-
-  Lemma fsetUs_cons (K : choiceType) (x : K) s L :
-    x \in fsetUs (s :: L) = (x \in s) || (x \in fsetUs L).
-  Proof.
-    rewrite /fsetUs/=.
-    elim: L fset0 => [s'|s' L Ih s'']/=; first (by rewrite in_fsetU orbC).
-    by rewrite fsetUC fsetUA Ih fsetUC.
-  Qed.
-
   Open Scope fset_scope.
-  Fixpoint g_fvar A (G : g_ty A) : {fset atom} :=
+  Fixpoint g_fvar (G : g_ty) : {fset atom} :=
     match G with
     | g_var v => fvar v
     | g_rec G => g_fvar G
-    | g_msg m p q Ks => fsetUs [seq g_fvar K.cnt | K <- Ks]
+    | g_msg p q Ks => fsetUs [seq g_fvar K.cnt | K <- Ks]
     | g_end => fset0
     end.
 
@@ -201,50 +186,53 @@ Section Syntax.
     (x \notin fsetUs l) = all (fun s => x \notin s) l.
   Proof. by rewrite in_fold_has -all_predC. Qed.
 
-  Fixpoint g_fbvar A (d : nat) (G : g_ty A) : {fset nat} :=
+  Fixpoint g_fbvar (d : nat) (G : g_ty) : {fset nat} :=
     match G with
     | g_var v => fbvar d v
     | g_rec G => g_fbvar d.+1 G
-    | g_msg m p q Ks => fsetUs [seq g_fbvar d K.cnt | K <- Ks]
+    | g_msg p q Ks => fsetUs [seq g_fbvar d K.cnt | K <- Ks]
     | g_end => fset0
     end.
 
-  Definition g_lc A (G : g_ty A) := g_fbvar 0 G = fset0.
+  Definition g_lc (G : g_ty) := g_fbvar 0 G = fset0.
 
-  Lemma in_gfvar_gfv A (a a' : atom) : (a \in g_fvar (A:=A) (gfv a')) = (a == a').
+  Definition g_closed (G : g_ty) :=
+    (g_fbvar 0 G == fset0) && (g_fvar G == fset0).
+
+  Lemma in_gfvar_gfv (a a' : atom) : (a \in g_fvar (gfv a')) = (a == a').
   Proof.
     rewrite /g_fvar; case: fset1P=>[->|].
     - by rewrite eq_refl.
     - by move=> /eqP/negPf->.
   Qed.
 
-  Lemma gopen_gfv A n X (a : atom) : g_open n X (A:=A) (gfv a) = gfv a.
+  Lemma gopen_gfv n X (a : atom) : g_open n X (gfv a) = gfv a.
   Proof. by []. Qed.
 
-  Lemma gclose_gfv A n X (a : atom) :
-    g_close (A:=A) X n (gfv a) = if X == a then (gbv n) else (gfv a).
-  Proof. by rewrite /g_close/close (fun_if (@g_var A)). Qed.
+  Lemma gclose_gfv n X (a : atom) :
+    g_close X n (gfv a) = if X == a then (gbv n) else (gfv a).
+  Proof. by rewrite /g_close/close (fun_if g_var). Qed.
 
-  Lemma g_open_close A X (G : g_ty A) n : X \notin g_fvar G -> {n <~ X}{n ~> gfv X}G = G.
+  Lemma g_open_close X (G : g_ty) n : X \notin g_fvar G -> {n <~ X}{n ~> gfv X}G = G.
   Proof.
     elim/gty_ind1: G n =>//.
     - by move=> v d /= H; rewrite open_fun /= (open_close d H).
     - move=> G Ih d; rewrite /g_fvar -/(g_fvar _)=>/Ih-{Ih}Ih.
       by rewrite -[in RHS](Ih d.+1).
-    - move=> m p q Ks Ih n /= H; rewrite -map_comp/comp/=; congr g_msg.
+    - move=> p q Ks Ih n /= H; rewrite -map_comp/comp/=; congr g_msg.
       elim: Ks H Ih => {p} {q} [//|/=[l [t G]] Ks Ih].
       rewrite fsetUs_cons negb_or /= =>/andP-[X_G X_KS] IhKs.
       rewrite (IhKs (l, (t, G)) (or_introl (Logic.eq_refl _)) n X_G) Ih //.
       by move=> K KKs r H; apply: IhKs =>//; right.
   Qed.
 
-  Lemma g_close_open A n X (G : g_ty A) : n \notin g_fbvar 0 G -> {n ~> gfv X}{n <~ X}G = G.
+  Lemma g_close_open n X (G : g_ty) : n \notin g_fbvar 0 G -> {n ~> gfv X}{n <~ X}G = G.
   Proof.
     move: {1 3}n (add0n n)=>n0; elim/gty_ind2: G 0 n =>///=.
     - by move=> v n n1 <- H; rewrite addnC open_fun close_open.
     - move=> G Ih d n Eq n_in; congr g_rec; apply: (Ih d.+1)=>//.
       by rewrite -Eq.
-    - move=> m p q Ks /Fa_lift-Fa d n Eq; rewrite notin_fold_all !all_map /preim/=.
+    - move=> p q Ks /Fa_lift-Fa d n Eq; rewrite notin_fold_all !all_map /preim/=.
       move: (Fa d)=>{Fa}/Fa_lift/(_ n)/Fa_lift/(_ Eq)-Fa.
       move=>/forallbP/(Fa_conj Fa){Fa}.
       rewrite /SimplPred/= =>/Fa_app/Fa_map_eq-Ih.
@@ -253,32 +241,67 @@ Section Syntax.
   Qed.
   Close Scope fset_scope.
 
-  Lemma g_depth_open A (G : g_ty A) X : depth_gty G = depth_gty (G^X).
+  Lemma g_depth_open (G : g_ty) X : depth_gty G = depth_gty (G^X).
   Proof.
     move: 0; elim/gty_ind2: G=>/=//.
     + by move=>v n; rewrite open_fun.
     + by move=> G Ih n; rewrite (Ih n.+1).
-    + move=> _ _ _ Gs /Fa_lift-Ih n; move: (Ih n) => {Ih}/Fa_map_eq.
+    + move=> _ _ Gs /Fa_lift-Ih n; move: (Ih n) => {Ih}/Fa_map_eq.
       rewrite -map_comp /comp/=.
       by elim: Gs=>[//|/=[l G] Gs Ih []<- /Ih-{Ih}[<-]].
   Qed.
 
+  Lemma gfbvar_next n G :
+    g_fbvar n G == fset0 ->
+    g_fbvar n.+1 G = fset0.
+  Proof.
+    elim/gty_ind1: G n=>[//|v|G Ih|p q Ks Ih] n/=.
+    - case: v=>//= m H; case: ifP=>// n_m; move: H.
+      by move: (leq_trans (leqnSn n) n_m)=>->; rewrite -cardfs_eq0 cardfs1.
+    - by apply: Ih.
+    - rewrite fsetUs_fset0 member_map=>H; apply/eqP.
+      by rewrite fsetUs_fset0 member_map=> K M; move: (Ih K M n (H K M))=>->.
+  Qed.
+
+  Lemma gopen_closed G :
+    g_closed (g_rec G) ->
+    g_closed (g_open 0 (g_rec G) G).
+  Proof.
+    rewrite/g_closed/==>/andP-[G_fbv /eqP-G_fv]; apply/andP; split=>[{G_fv}|{G_fbv}].
+    + have: g_fbvar 0 (g_rec G) == fset0 by [].
+      move: (g_rec G) => G' G'0.
+      elim/gty_ind1: G 0 G'0 G_fbv=>[//|v|G Ih|p q Ks Ih] n G'0/=.
+      - case: v=>[//|/= m]; case: ifP; first by rewrite -cardfs_eq0 cardfs1//.
+        case: ifP=>[/eqP<-//|/=]; case: ifP=>//.
+        by rewrite ltn_neqAle (rwP negPf)=>->->.
+      - by apply: (Ih n.+1); rewrite gfbvar_next.
+      - rewrite -map_comp/comp/=; move=>/fsetUs_fset0/member_map-H.
+        by apply/fsetUs_fset0/member_map=>K M; apply: Ih=>//; apply: H.
+    + move: G_fv=>/eqP-G_fv; have: g_fvar (g_rec G) == fset0 by [].
+      move: (g_rec G) => G' G'_fv.
+      elim/gty_ind1: G 0 G_fv =>[//|v |G Ih | p q Ks Ih] n /=.
+      - by case v=>//; case =>[|m]//=; case: ifP.
+      - by apply: Ih.
+      - rewrite -map_comp/comp !fsetUs_fset0 !member_map=> H K M.
+        by apply: Ih => //; apply: H.
+  Qed.
+
   (* Induction scheme that takes into account that g_rec must be opened *)
   Lemma gty_ind3 :
-    forall (A :eqType) (P : g_ty A -> Type),
+    forall (P : g_ty -> Type),
       P g_end ->
       (forall v, P (g_var v)) ->
       (forall G, (forall X (s : {fset atom}), X \notin s -> P (G ^ X)) ->
                  P (g_rec G)) ->
-      (forall m p q Ks, (forall K, K \in Ks -> P K.cnt) -> P (g_msg m p q Ks)) ->
-      forall g : g_ty A, P g.
+      (forall p q Ks, (forall K, K \in Ks -> P K.cnt) -> P (g_msg p q Ks)) ->
+      forall g : g_ty, P g.
   Proof.
-    move=> A P P_end P_var P_rec P_msg G.
+    move=> P P_end P_var P_rec P_msg G.
     move: {-1}(depth_gty G) (leqnn (depth_gty G))=> n; move: n G; elim.
     + by case.
     + move=>n Ih; case=>///=.
       - by move=> G dG; apply: P_rec => X S _; apply: Ih; rewrite -g_depth_open.
-      - move=>m p q Ks dKs; apply: P_msg=>K /(map_f (fun X => depth_gty X.cnt))/=.
+      - move=>p q Ks dKs; apply: P_msg=>K /(map_f (fun X => depth_gty X.cnt))/=.
         move=>/in_maximum_leq-dG; move: (leq_trans dG dKs)=>{dG} {dKs}.
         by apply: Ih.
   Qed.
@@ -287,38 +310,44 @@ End Syntax.
 
 Section Semantics.
 
-  Definition rg_ty := g_ty (option lbl).
+  CoInductive rg_ty :=
+  | rg_end
+  | rg_msg (a : option lbl) (p : role) (q : role) (Ks : seq (lbl * (mty * rg_ty))).
+
+  CoInductive GUnroll : g_ty -> rg_ty -> Prop :=
+  | gu_end : GUnroll g_end rg_end
+  | gu_rec G G' : GUnroll (g_open 0 (g_rec G) G) G' -> GUnroll (g_rec G) G'
+  | gu_msg p q Ks Ks' : GUnrollAll Ks Ks' ->
+                        GUnroll (g_msg p q Ks) (rg_msg None p q Ks')
+  with GUnrollAll
+       : seq (lbl * (mty * g_ty)) -> seq (lbl * (mty * rg_ty)) -> Prop :=
+  | gu_nil : GUnrollAll [::] [::]
+  | gu_cons l t G G' Ks Ks' :
+      GUnroll G G' ->
+      GUnrollAll Ks Ks' ->
+      GUnrollAll ((l, (t, G)) :: Ks) ((l, (t, G')) :: Ks')
+  .
 
   Open Scope mpst_scope.
-
-  Definition conflict a (m : option lbl) p q :=
-    match m with
-    | None => ~~ ((subject a == p) || (subject a == q))
-    | Some _ => subject a != q
-    end.
 
   Inductive step : act -> rg_ty -> rg_ty -> Prop :=
   (* Basic rules *)
   | st_send lb p q Ks t G :
-      lookup lb Ks == Some (t, G) ->
-      step (a_send p q lb t) (g_msg None p q Ks) (g_msg (Some lb) p q Ks)
+      lookup lb Ks = Some (t, G) ->
+      step (a_send p q lb t) (rg_msg None p q Ks) (rg_msg (Some lb) p q Ks)
   | st_recv lb p q Ks t G :
-      lookup lb Ks == Some (t, G) ->
-      step (a_recv p q lb t) (g_msg (Some lb) p q Ks) G
-
+      lookup lb Ks = Some (t, G) ->
+      step (a_recv p q lb t) (rg_msg (Some lb) p q Ks) G
   (* Struct *)
   | st_amsg1 a p q Ks Ks' :
       subject a != p ->
       subject a != q ->
       step_all a Ks Ks' ->
-      step a (g_msg None p q Ks) (g_msg None p q Ks')
+      step a (rg_msg None p q Ks) (rg_msg None p q Ks')
   | st_amsg2 l a p q Ks Ks' :
       subject a != q ->
       step_only l a Ks Ks' ->
-      step a (g_msg (Some l) p q Ks) (g_msg (Some l) p q Ks')
-  | st_rec l G G' :
-      step l (g_open 0 G (g_rec G)) G' ->
-      step l (g_rec G) G'
+      step a (rg_msg (Some l) p q Ks) (rg_msg (Some l) p q Ks')
   with
   step_all : act ->
              seq (lbl * (mty * rg_ty)) ->
@@ -351,7 +380,7 @@ Section Semantics.
   with steponly_ind1 := Induction for step_only Sort Prop.
 
   CoInductive g_lts : trace -> rg_ty -> Prop :=
-  | eg_end : g_lts tr_end (@g_end (option lbl))
+  | eg_end : g_lts tr_end rg_end
   | eg_trans a t G G' :
       step a G G' ->
       g_lts t G' ->
