theories/Projection.v
@@ -12,7 +12,7 @@ Require Import MPST.Local.
 Require Import MPST.Session.
 Require Import MPST.Actions.
 
-Section Project.
+Section IProject.
 
   Open Scope mpst_scope.
 
@@ -77,7 +77,6 @@ Section Project.
       end.
   Proof. by []. Qed.
 
-  Notation g_ty := (g_ty unit).
   Notation Lfv a := (l_var (fv a)).
   Notation lbv n := (l_var (bv _ n)).
 
@@ -87,10 +86,10 @@ Section Project.
     | g_var v => Some (l_var v)
     | g_rec G =>
       match project G r with
-      | Some L => if L == lbv 0 then None else Some (l_rec L)
+      | Some L => Some (if L == lbv 0 then l_end else l_rec L)
       | None => None
       end
-    | g_msg _ p q Ks =>
+    | g_msg p q Ks =>
       match (fix proj_all Ks r :=
                match Ks with
                | [::] => Some [::]
@@ -119,8 +118,8 @@ Section Project.
                end
     end.
 
-  Lemma project_msg a p q Ks r
-    : project (g_msg a p q Ks) r =
+  Lemma project_msg p q Ks r
+    : project (g_msg p q Ks) r =
       match prj_all Ks r with
       | Some Ks' => if p == q then None
                    else if p == r then Some (l_msg l_send q Ks')
@@ -144,6 +143,550 @@ Section Project.
     - by move=> /(Ih LKs Ksp K0)-[L [L_LKs PrjL]]; exists L; split=>//=; right.
   Qed.
 
+  Lemma prjall_some2 p Ks Ks' :
+    prj_all Ks p == Some Ks' ->
+    forall K, member K Ks' ->
+              exists G, member (K.lbl, (K.mty, G)) Ks /\
+                        project G p = Some K.cnt.
+  Proof.
+    elim: Ks' => [|K Ks' Ih]//= in Ks *.
+    case: Ks=>// Kg Ks/=.
+    case Kgp: (project Kg.cnt p) => [Lp|//].
+    case Ksp: (prj_all Ks p) => [Ks''|//]; move: Ksp=>/eqP-Ksp.
+    move=>/eqP-[[<-{K} EqKs'']]; move: EqKs'' Ksp=>->Ksp {Ks''}.
+    move=> K [->{K}|].
+    - by exists (Kg.cnt) =>/=; split=>//; left; case: Kg {Kgp} => l [t G].
+    - move=> M; move: (Ih Ks Ksp K M)=>[G [MG prjG]].
+      by exists G; split=>//; right.
+  Qed.
+
+  Definition full_project G p q :=
+    match project G p with
+    | Some L => partial_proj L q
+    | None => None
+    end.
+
+  Definition fullproj_all Ks p q :=
+    match prj_all Ks p with
+    | Some LKs => pprj_all LKs q
+    | None => None
+    end.
+
+  Lemma fullproject_some p q G L S
+    : project G p == Some L -> partial_proj L q == Some S ->
+      full_project G p q = Some S.
+  Proof. by rewrite /full_project =>/eqP-> /eqP. Qed.
+
+  Lemma def_fprojall p q G L S
+    : prj_all G p == Some L -> pprj_all L q == Some S ->
+      fullproj_all G p q = Some S.
+  Proof. by rewrite /fullproj_all =>/eqP-> /eqP. Qed.
+
+
+  Lemma dualproj_msg Ks p q Ks0 Ks1 S S' a1 a2 :
+    (forall s s0 : seq (lbl * (mty * s_ty)),
+        fullproj_all Ks p q == Some s ->
+        fullproj_all Ks q p == Some s0 ->
+        s0 = [seq (x.lbl, (x.mty, dual x.cnt)) | x <- s]) ->
+    a2 == dual_act a1 ->
+    prj_all Ks p = Some Ks0 ->
+    prj_all Ks q = Some Ks1 ->
+    partial_proj (l_msg a1 q Ks0) q == Some S ->
+    partial_proj (l_msg a2 p Ks1) p == Some S' ->
+    S' = dual S.
+  Proof.
+    move=> Ih /eqP-a12 Lp Lq; rewrite !partialproj_all !eq_refl.
+    case Kspq: (pprj_all Ks0) => [Ks0'|//].
+    case Ksqp: (pprj_all Ks1) => [Ks1'|//].
+    move=> /eqP-[<-]/eqP-[<-]/=; congr s_msg=>//.
+    by rewrite (Ih Ks0' Ks1') /fullproj_all ?Lp ?Kspq ?Lq ?Ksqp.
+  Qed.
+
+  Lemma merge_some (A : eqType)
+        (K : lbl * (mty * A))
+        (Ks : seq (lbl * (mty * A))) L
+    : merge K.cnt [seq K0.cnt | K0 <- Ks] == Some L -> K.cnt = L.
+  Proof. by elim: Ks=>[/eqP-[]//|K' Ks Ih/=]; case:ifP. Qed.
+
+  Lemma merge_pprj L' Ks L p S
+    : merge L' [seq K.cnt | K <- Ks] == Some L -> partial_proj L p == Some S ->
+      exists Ks', pprj_all Ks p = Some Ks' /\
+                  merge S [seq K.cnt | K <- Ks'] = Some S.
+  Proof.
+    elim: Ks=>[_|K' Ks Ih]/=; first (by exists [::]; split); move: Ih.
+    case: ifP=>///eqP<- Ih M_L'; move: (merge_some M_L')=>-> /eqP-L_S.
+    rewrite L_S; move: L_S=>/eqP-L_S; move: (Ih M_L' L_S) => [Ks' [Ksp M_S]].
+    by exists ((K'.lbl, (K'.mty, S)):: Ks'); rewrite Ksp /= eq_refl M_S.
+  Qed.
+
+  Lemma mergeall_pprj Ks L p S
+    : merge_all [seq K.cnt | K <- Ks] == Some L -> partial_proj L p == Some S ->
+      exists Ks', pprj_all Ks p = Some Ks' /\
+                  merge_all [seq K.cnt | K <- Ks'] = Some S.
+  Proof.
+    case: Ks=>[//|K Ks]/=; move=> H; move: (merge_some H)=>KL.
+    move: KL H=>-> H /eqP-L_S; rewrite L_S; move: L_S=>/eqP-L_S.
+    move: (merge_pprj H L_S)=>[Ks' [Ksp M_S]].
+    by exists ((K.lbl, (K.mty, S)) :: Ks'); rewrite Ksp/= M_S.
+  Qed.
+
+  Lemma fun_mergeall (A B : eqType) (f : A -> B) (Ks : seq (lbl * (mty * A))) X
+    : injective f ->
+      merge_all [seq f x.cnt | x <- Ks] == Some (f X) ->
+      merge_all [seq x.cnt | x <- Ks] == Some X.
+  Proof.
+    case: Ks=>[//|K Ks/=] I; elim: Ks=>[|K' Ks]//=.
+    - by move=>/eqP-[/I->].
+    - by move=> Ih; case: ifP=>///eqP-[/I->]; rewrite eq_refl=>/Ih.
+  Qed.
+
+  Lemma dualproj_all Ks p q Ks0 Ks1 S S' s a :
+    (forall s s0 : seq (lbl * (mty * s_ty)),
+        fullproj_all Ks p q == Some s ->
+        fullproj_all Ks q p == Some s0 ->
+        s0 = [seq (x.lbl, (x.mty, dual x.cnt)) | x <- s]) ->
+    prj_all Ks p = Some Ks0 ->
+    prj_all Ks q = Some Ks1 ->
+    (s == q) = false ->
+    partial_proj (l_msg a s Ks0) q == Some S ->
+    match merge_all [seq K.cnt | K <- Ks1] with
+    | Some L => partial_proj L p
+    | None => None
+    end == Some S' ->
+    S' = dual S.
+  Proof.
+    move=> Ih Ksp Ksq s_neq_q; rewrite !partialproj_all s_neq_q.
+    case Kspq: (pprj_all Ks0) => [Ks0'|//]; move => EqS.
+    case Ksqp: (merge_all [seq K.cnt | K <- Ks1]) => [L'|//].
+    move: Ksqp=>/eqP-Ksqp  L'S'.
+    move: (mergeall_pprj Ksqp L'S')=>[Ks' [/eqP-Ks1p /eqP-H]]; move: H EqS.
+    rewrite (Ih Ks0' Ks' ) /fullproj_all ?Ksp ?Kspq ?Ksq//.
+    rewrite -map_comp /comp/= -{1}(dualK S').
+    by move=>/(fun_mergeall dualI)/eqP-> /eqP-[<-]; rewrite dualK.
+  Qed.
+
+  Lemma dualproj_all2 Ks p q Ks0 Ks1 S S' s a :
+    (forall s s0 : seq (lbl * (mty * s_ty)),
+        fullproj_all Ks p q == Some s ->
+        fullproj_all Ks q p == Some s0 ->
+        s0 = [seq (x.lbl, (x.mty, dual x.cnt)) | x <- s]) ->
+    prj_all Ks p = Some Ks0 ->
+    prj_all Ks q = Some Ks1 ->
+    (s == p) = false ->
+    match merge_all [seq K.cnt | K <- Ks0] with
+    | Some L => partial_proj L q
+    | None => None
+    end == Some S ->
+    partial_proj (l_msg a s Ks1) p == Some S' ->
+    S' = dual S.
+  Proof.
+    move=> Ih Ksp Ksq s_neq_q; rewrite !partialproj_all s_neq_q.
+    case Kspq: (pprj_all Ks1) => [Ks0'|//].
+    case Ksqp: (merge_all [seq K.cnt | K <- Ks0]) => [L'|//].
+    move: Ksqp=>/eqP-Ksqp  L'S'.
+    move: (mergeall_pprj Ksqp L'S')=>[Ks' [/eqP-Ks1p /eqP-H]]; move: H.
+    rewrite (Ih Ks' Ks0' ) /fullproj_all ?Ksp ?Ksq ?Kspq//.
+    rewrite -map_comp /comp/= -{1}(dualK S').
+    move=>H1 /(fun_mergeall dualI)/eqP-H2; move: H2 H1.
+    by move=>->/eqP-[<-]; rewrite dualK.
+  Qed.
+
+  Lemma fprojall_eq Ks p q Ks0 Ks1
+    : (forall K, member K Ks ->
+                 forall S S', full_project K.cnt p q == Some S ->
+                              full_project K.cnt q p == Some S' ->
+                              S' = dual S) ->
+      fullproj_all Ks p q == Some Ks0 ->
+      fullproj_all Ks q p == Some Ks1 ->
+      Ks1 = [seq (x.lbl, (x.mty, dual x.cnt)) | x <- Ks0].
+  Proof.
+    elim: Ks =>[|K Ks Ih] /= in Ks0 Ks1 *.
+    - by move=> H; rewrite /fullproj_all/==>/eqP-[<-]/eqP-[<-].
+    - move=> H; rewrite /fullproj_all/=.
+      case Kp: (project K.cnt p)=>[Lp|]//; case Ksp: (prj_all Ks p)=>[Lsp|]//=.
+      case Ep: (partial_proj Lp q)=>[Sp|]//; case Esp: (pprj_all Lsp q)=>[Ssp|]//=.
+      case Kq: (project K.cnt q)=>[Lq|]//; case Ksq: (prj_all Ks q)=>[Lsq|]//=.
+      case Eq: (partial_proj Lq p)=>[Sq|]//; case Esq: (pprj_all Lsq p)=>[Ssq|]//=.
+      move=>/eqP-[<-]/eqP-[<-]/=.
+      rewrite -(H K _ Sp Sq) /full_project ?Kp ?Ep ?Kq ?Eq //; last (by left).
+      congr cons; apply/Ih; rewrite /fullproj_all ?Ksp ?Esp ?Ksq ?Esq//.
+      by move=> K0 K0Ks; apply/H; right.
+  Qed.
+
+  Lemma prjall_merge p Ks KsL L :
+    prj_all Ks p == Some KsL ->
+    merge_all [seq K0.cnt | K0 <- KsL] == Some L ->
+    forall K, member K Ks -> project K.cnt p == Some L.
+  Proof.
+    case: KsL=>//= Kl KsL; case: Ks=>//= Kg Ks.
+    case Kg_p: project => [Lp | //]; case Ks_p: prj_all => [Ksp | //]/=.
+    move=> Eq; move: Eq Ks_p => /eqP-[<-->] /eqP-Prj Mrg {Kl Ksp}.
+    move:Mrg (merge_some Mrg)=>/=Mrg Eq; move: Eq Mrg Kg_p=>->Mrg /eqP-Kg_p.
+    move=> K [->//|]; move: Prj Mrg K {Lp Kg_p Kg}.
+    elim: Ks KsL=>//= Kg Ks Ih KsL.
+    case Kg_p: project => [Lp | //]; case Ks_p: prj_all => [Ksp | //]/=.
+    move=> Eq; move: Eq Ih Ks_p Kg_p=>/eqP-[<-]//= Ih /eqP-Prj.
+    case: ifP=>[/eqP-> {Lp}|//] /eqP-Kg_p Mrg K [->//|].
+    by move: Prj=>/Ih/(_ Mrg K).
+  Qed.
+
+  Lemma project_var_notin p G v L :
+    (L == l_end) || (L == l_var v) ->
+    project G p == Some L ->
+    p \notin participants G.
+  Proof.
+    elim/gty_ind1: G => [|v'|G Ih|q r Ks Ih]// in L v *.
+    - move: Ih=>/=; case: (project G p)=>[Lp|//] Ih.
+      move=>/orP-[/eqP->|/eqP->]; case: ifP=>[/eqP-Lp_var|]//.
+      move: Lp_var Ih =>-> /(_ (lbv 0) (bv _ 0))-Ih _.
+      by apply:Ih; rewrite eq_refl // orbC.
+    - rewrite project_msg; case E: (prj_all _ _)=>[KsL|//]; move: E=>/eqP-E/=.
+      case: ifP=>[//|/(rwP negPf)-q_ne_r].
+      case: ifP=>[/eqP->/orP-[/eqP->|/eqP->]//|/(rwP negPf)-q_ne_p].
+      case: ifP=>[/eqP->/orP-[/eqP->|/eqP->]//|/(rwP negPf)-r_ne_p].
+      do 2 rewrite in_cons negb_or; move=> L_end_var M_some.
+      do 2 rewrite eq_sym ?q_ne_p /= ?r_ne_p /=; move: M_some.
+      move: E=>/prjall_merge-E /E-Prjall.
+      apply/flatten_mapP=>[[Kg /memberP-M]].
+      by apply/negP; apply: (Ih _ M L v L_end_var); apply: Prjall.
+  Qed.
+
+  Lemma projectmsg_var p r s Ks :
+    project (g_msg r s Ks) p == Some (lbv 0) ->
+    r != p /\ s != p /\ r != s /\
+    (forall K, member K Ks -> project K.cnt p == Some (lbv 0)).
+  Admitted.
+
+  Lemma pprjall_merge p Ks KsL L :
+    pprj_all Ks p == Some KsL ->
+    merge_all [seq K0.cnt | K0 <- KsL] == Some L ->
+    forall K, member K Ks -> partial_proj K.cnt p == Some L.
+  Proof.
+    (*
+    case: KsL=>//= Kl KsL; case: Ks=>//= Kg Ks.
+    case Kg_p: project => [Lp | //]; case Ks_p: prj_all => [Ksp | //]/=.
+    move=> Eq; move: Eq Ks_p => /eqP-[<-->] /eqP-Prj Mrg {Kl Ksp}.
+    move:Mrg (merge_some Mrg)=>/=Mrg Eq; move: Eq Mrg Kg_p=>->Mrg /eqP-Kg_p.
+    move=> K [->//|]; move: Prj Mrg K {Lp Kg_p Kg}.
+    elim: Ks KsL=>//= Kg Ks Ih KsL.
+    case Kg_p: project => [Lp | //]; case Ks_p: prj_all => [Ksp | //]/=.
+    move=> Eq; move: Eq Ih Ks_p Kg_p=>/eqP-[<-]//= Ih /eqP-Prj.
+    case: ifP=>[/eqP-> {Lp}|//] /eqP-Kg_p Mrg K [->//|].
+    by move: Prj=>/Ih/(_ Mrg K).
+*)
+  Admitted.
+
+  Lemma pprjall_some p Ks Ks' :
+    pprj_all Ks p == Some Ks' ->
+    forall K,
+      member K Ks ->
+      exists L, member (K.lbl, (K.mty, L)) Ks' /\ partial_proj K.cnt p = Some L.
+  Admitted.
+
+  Lemma pproj_var p q G Lq Sq :
+    project G p == Some (lbv 0) ->
+    project G q == Some Lq ->
+    partial_proj Lq p == Some Sq ->
+    Sq = sbv 0.
+  Proof.
+    elim/gty_ind1: G =>[//|v//=|G Ih//=|r s Ks Ih] in Lq Sq *.
+    - by move=>/eqP-[->]/eqP-[<-]/=/eqP-[<-].
+    - by case: project=>//L; case: ifP.
+    - move=> /projectmsg_var-[r_ne_p [s_ne_p [r_ne_s Ksp]]].
+      rewrite project_msg; case Eq: prj_all=>[KsL|//]; move: Eq=>/eqP-Prj_Ks.
+      rewrite (negPf r_ne_s); do ! case: ifP=>[_ /eqP-[<-]|_].
+      * rewrite partialproj_all (negPf s_ne_p); case E: pprj_all=>[KsS|//] Mrg.
+        move: E=>/eqP-E.
+        admit.
+        (*
+        suff: exists K, member K Ks.
+        move=>[Kg M].
+        case: Ks Prj_Ks{Ksp Ih} M=>[|Kl Ks _]; last (by exists Kl; left).
+        admit.
+         *)
+      * rewrite partialproj_all (negPf r_ne_p); case E: pprj_all=>[KsS|//] Mrg.
+        admit.
+      * move=> Mrg PPrj.
+        suff : exists K, member K Ks by
+              move=>[K M]; move: Mrg=>/(prjall_merge Prj_Ks)-Ksq{Prj_Ks};
+                      move: Ih=>/(_ K M _ _ (Ksp _ M) (Ksq _ M) PPrj)-Ih.
+        case: Ks Prj_Ks {Ih Ksp}=>[//=|K Ks _]; last (by exists K; left).
+        by move=>/eqP-[Eq]; move: Eq Mrg=><-.
+  Admitted.
+
+  Lemma all_compat G S S' p q :
+    p != q ->
+    full_project G p q == Some S ->
+    full_project G q p == Some S' ->
+    S' = dual S.
+  Proof.
+    move=>/negPf-p_neq_q.
+    elim/gty_ind1: G => [|v|G Ih| r s Ks Ih] in S S' *.
+    - by do ! (move=>/eqP-[<-]).
+    - by do ! (move=>/eqP-[<-]).
+    - rewrite /full_project/=.
+      case Ep: project=>[Lp|//]; case Eq: project=>[Lq|//].
+      move: Ep Eq; do ! case: ifP=>[/eqP->//=|//=].
+      * by move=> _ _ /eqP-[<-] /eqP-[<-].
+      * case Eq: partial_proj=>[Sq|]//; move: Eq=>/eqP-Eq.
+        move=>_ /eqP-Gp_var /eqP-Gq_Lq; move: (pproj_var Gp_var Gq_Lq Eq)=>->.
+        by rewrite eq_refl=>/eqP-[<-] /eqP-[<-].
+      * case Eq: partial_proj=>[Sq|]//; move: Eq=>/eqP-Eq.
+        move=>_ /eqP-Gp /eqP-Gq; move: (pproj_var Gq Gp Eq)=>->.
+        by rewrite eq_refl=>/eqP-[<-] /eqP-[<-].
+      * case Ep: partial_proj=>[Sp|]//; move: Ep=>/eqP-Ep.
+        case Eq: partial_proj=>[Sq|]//; move: Eq=>/eqP-Eq.
+        move=>_ _ /eqP-Prj_p /eqP-Prj_q.
+        move: Prj_p Ep =>/fullproject_some-Prj_p /Prj_p/eqP/Ih-{Prj_p Ih}Ih.
+        move: Prj_q Eq =>/fullproject_some-Prj_q /Prj_q/eqP/Ih-{Prj_q Ih}Ih.
+        move: Ih; case: ifP=>[/eqP->->//= /eqP-[<-] /eqP-[<-]//|H -> /eqP-[<-]].
+        by move: H; rewrite -{1}(dualK Sp); case: ifP=>[/eqP->//|_ _ /eqP-[<-]].
+    - move: Ih=>/fprojall_eq-Ih; rewrite /full_project !project_msg.
+      case Ksp: (prj_all Ks) => [Ks0|//]; case Ksq: (prj_all Ks) => [Ks1|//].
+      case: ifP=>// -r_neq_s.
+      do ! (case: ifP=>[/eqP->|]//; rewrite ?p_neq_q ?r_neq_s //).
+      * by apply: (dualproj_msg Ih).
+      * by apply: (dualproj_all Ih).
+      * by move=> _; apply: (dualproj_msg Ih).
+      * by move=> r_neq_q _; apply: (dualproj_all Ih).
+      * by move=> s_neq_p _; apply: (dualproj_all2 Ih).
+      * by move=> _ _ r_neq_p; apply: (dualproj_all2 Ih).
+      * case M_Ks0: (merge_all [seq K.cnt | K <- Ks0]) => [L'|//].
+        case M_Ks1: (merge_all [seq K.cnt | K <- Ks1]) => [L|//].
+        move: M_Ks0 M_Ks1 =>/eqP-M_Ks0 /eqP-M_Ks1 _ _ _ _ L'S LS'.
+        move: (mergeall_pprj M_Ks0 L'S)=>[Ks' [/eqP-Ks0q /eqP-H]]; move: H.
+        move: (mergeall_pprj M_Ks1 LS')=>[Ks'' [/eqP-Ks1p /eqP-H]]; move: H.
+        rewrite (Ih Ks' Ks'') /fullproj_all ?Ksp ?Ksq // -map_comp/comp/=.
+        rewrite -{1}(dualK S'); move=>/(fun_mergeall dualI)/eqP->/eqP-[<-].
+        by rewrite dualK.
+  Qed.
+
+End IProject.
+
+Section CProject.
+
+  CoInductive EqL : rl_ty -> rl_ty -> Prop :=
+  | el_end : EqL rl_end rl_end
+  | el_msg a p Ks1 Ks2 :
+      AllEqL Ks1 Ks2 ->
+      EqL (rl_msg a p Ks1) (rl_msg a p Ks2)
+  with AllEqL : seq (lbl * (mty * rl_ty)) ->
+                seq (lbl * (mty * rl_ty)) ->
+                Prop :=
+  | el_nil : AllEqL [::] [::]
+  | el_cons l t L1 L2 Ks1 Ks2 :
+      EqL L1 L2 ->
+      AllEqL Ks1 Ks2 ->
+      AllEqL ((l, (t, L1)) :: Ks1) ((l, (t, L2)) :: Ks2).
+
+  Inductive Merge : seq (lbl * (mty * rl_ty)) -> rl_ty -> Prop :=
+  | m_nil l t L : Merge [:: (l, (t, L))] L
+  | m_cons l t L1 L2 Ks :
+      EqL L1 L2 ->
+      Merge Ks L2 ->
+      Merge ((l, (t, L1)) :: Ks) L2.
+
+  CoInductive Project (p : role) : rg_ty -> rl_ty -> Prop :=
+  | prj_end : Project p rg_end rl_end
+  | prj_send1 q KsG KsL :
+      p != q ->
+      ProjectAll p KsG KsL ->
+      Project p (rg_msg None p q KsG) (rl_msg l_send q KsL)
+  | prj_send2 l t q KsG KsL L :
+      p != q ->
+      ProjectAll p KsG KsL ->
+      lookup l KsL = Some (t, L) ->
+      Project p (rg_msg (Some l) p q KsG) L
+  | prj_recv o q KsG KsL :
+      p != q ->
+      ProjectAll p KsG KsL ->
+      Project p (rg_msg o q p KsG) (rl_msg l_recv q KsL)
+  | prj_mrg o q r KsG KsL L :
+      q != r ->
+      p != q ->
+      p != r ->
+      ProjectAll p KsG KsL ->
+      Merge KsL L ->
+      Project p (rg_msg o q r KsG) L
+  with ProjectAll (p : role) :
+         seq (lbl * (mty * rg_ty)) ->
+         seq (lbl * (mty * rl_ty)) ->
+         Prop :=
+  | prj_nil  : ProjectAll p [::] [::]
+  | prj_cons l t G L KsG KsL :
+      Project p G L ->
+      ProjectAll p KsG KsL ->
+      ProjectAll p ((l, (t, G)) :: KsG) ((l, (t, L)) :: KsL)
+  .
+
+  Lemma project_rec G r L :
+    project G r == Some L ->
+    ((L == l_var (bv _ 0)) = false) ->
+    project (g_rec G) r = Some (l_rec L).
+  Proof. by move=>/=/eqP-[->] ->. Qed.
+
+  Lemma gclosed_lclosed G r L :
+    g_closed G ->
+    project G r == Some L ->
+    l_closed L.
+  Proof.
+    rewrite /g_closed/l_closed; elim/gty_ind1: G L 0 =>[|v|G Ih|p q Ks Ih] L n.
+    - by move=> _ /eqP-[<-].
+    - case: v=> [a|m /andP-[]]//=; first by rewrite -cardfs_eq0 cardfs1.
+      case: ifP; first by rewrite -cardfs_eq0 cardfs1.
+      by move=> H _ _ /eqP-[<-]/=; rewrite H.
+    - move: Ih=>/=; case Eq: (project G r) =>[Lr|//].
+      move=> /(_ Lr n.+1)-Ih; move=>/Ih/(_ (eq_refl _)).
+      by case: ifP=>// _ H /eqP-[<-].
+    - rewrite project_msg=>/=/andP-[H1 H2].
+      case Eq: (prj_all Ks r) => [Ks'|//]; case: ifP=>[//|p_neq_q]/=.
+      move: Eq=>/eqP-Eq.
+      case: ifP=>[p_eq_r /eqP-[<-]/=|p_neq_r].
+      * apply/andP; rewrite !fsetUs_fset0 !member_map in H1 H2 *=> H1 H2.
+        apply/all_and2 => K; apply/all_and2=> M; apply/andP.
+        move: (prjall_some2 Eq M) =>[G [M' /eqP-PrjG]].
+        by apply: (Ih _ M'); first by rewrite H1 // H2.
+      * case: ifP=>[q_eq_r /eqP-[<-]|q_neq_r /eqP].
+        + apply/andP; rewrite !fsetUs_fset0 !member_map in H1 H2 *=> H1 H2.
+          apply/all_and2 => K; apply/all_and2=> M; apply/andP.
+          move: (prjall_some2 Eq M) =>[G [M' /eqP-PrjG]].
+          by apply: (Ih _ M'); first by rewrite H1 // H2.
+        + case: Ks' Eq=>// Kl Ks' Eq /eqP/merge_some<- /=.
+          case: Ks Eq Ih H1 H2=>//= Kg Ks.
+          case Eqg: (project Kg.2.2 r)=>[Lk|//].
+          case EqKs: (prj_all Ks r)=>[Ks''|//].
+          rewrite !fsetUs_list=> /eqP-[[<- H2]] Ih /andP-[H3 H4] /andP-[H5 H6].
+          by apply: (Ih Kg)=>//=; [left|rewrite H3 H5|apply/eqP].
+  Qed.
+
+  Lemma prjall_open r n g l Ks Ks' :
+    (forall p : lbl * (mty * g_ty),
+      member p Ks ->
+      forall s : lty_eqType,
+        project p.2.2 r == Some s ->
+        project (g_open n g p.2.2) r = Some (l_open n l s)) ->
+    prj_all Ks r = Some Ks' ->
+    prj_all [seq (K.1, (K.2.1, g_open n g K.2.2)) | K <- Ks] r
+    = Some [seq (K.1, (K.2.1, l_open n l K.2.2)) | K <- Ks'].
+  Proof.
+    elim: Ks Ks' => [|K Ks Ih]; case=>[|K' Ks']//=.
+    - by case: (project K.2.2 r); case: (prj_all Ks r).
+    - move=> H. move: (H K (or_introl erefl)).
+      case: (project K.2.2 r) =>// L /(_ L (eq_refl _))->.
+      move: H=>/(_ _ (or_intror _))-H; move: Ih => /(_ _ H) {H}.
+      by case: (prj_all Ks r)=>[Ksr|//] /(_ Ksr erefl)-> [<-<-]/=.
+  Qed.
+
+  Lemma project_closed G r L :
+    project G r == Some L ->
+    g_closed (g_rec G) ->
+    ((L == l_var (bv _ 0)) = false) ->
+    project (g_open 0 (g_rec G) G) r = Some (l_open 0 (l_rec L) L).
+  Proof.
+    move=> H C L0; move: (project_rec H L0) => Hr; move: 0 {L0} (g_rec G) C (l_rec L) Hr.
+    elim/gty_ind1: G L H =>[|v|G Ih|p q Ks Ih] L.
+    - by move=>/eqP-[<-].
+    - move=> H; move: H =>/eqP-[<-] /= n G' C L'.
+      by case: v G' C=>//= m; case: ifP.
+    - move:Ih=>/=;case Eq:(project G r)=>[Lr|//].
+      move: Eq=> /eqP-Eq /(_ Lr (eq_refl _))-Ih.
+      case:ifP=>//H/eqP-[<-] n g cg l prj.
+      move: Ih=>/(_ n.+1 g cg l prj)->/=; move: prj=>/eqP-prj.
+      case: ifP=>//; move: (gclosed_lclosed cg prj) => cl.
+      case: Lr {Eq} H=>//=; case=>//= m; case: ifP; last by move=> _ ->.
+      move=> _ _ H; case: l cl {prj} H=>// v.
+      (*
+      rewrite /l_closed/=; case: v=>//= s /andP-[].
+      by rewrite -cardfs_eq0 cardfs1.
+       *)
+      admit.
+      admit.
+      admit.
+      admit.
+      admit.
+    - rewrite project_msg.
+      case Ksr: (prj_all Ks r) =>[Ks'|//].
+      case: ifP=>[//|p_neq_q].
+      case: ifP=>[/eqP-p_eq_r|p_neq_r].
+      * move=>/eqP-[<-]{L} n g cg l prj_g_l.
+        rewrite /g_open -/g_open  /l_open -/l_open.
+        rewrite project_msg p_neq_q p_eq_r eq_refl.
+        move: Ih => /(_ _ _ _ _ n g cg l prj_g_l)-Ih.
+        by move: (prjall_open Ih Ksr)=>->.
+      * case: ifP=>[/eqP-q_eq_r|q_neq_r].
+        + move=>/eqP-[<-]{L} n g cg l prj_g_l.
+          rewrite /g_open -/g_open  /l_open -/l_open.
+          rewrite project_msg p_neq_q p_neq_r q_eq_r eq_refl.
+          move: Ih => /(_ _ _ _ _ n g cg l prj_g_l)-Ih.
+          by move: (prjall_open Ih Ksr)=>->.
+        + move=> Mrg n g cg l prj; rewrite /g_open-/g_open project_msg.
+          rewrite p_neq_q p_neq_r q_neq_r.
+          move: Ih=>/(_ _ _ _ _ n g cg l prj)-Ih.
+          move: (prjall_open Ih Ksr)=>->; rewrite -map_comp/comp/=.
+          move: Mrg=>{Ksr}; case: Ks'=>//=K Ks'.
+          elim: Ks'=>//=; first by move=>/eqP-[->].
+          by move=> K' Ks' IhKs; case: ifP=>// /eqP->; rewrite eq_refl=>/IhKs.
+  Admitted.
+
+  (*
+  Fixpoint gunrollings n G :=
+    match n with
+    | n.+1 =>
+      match G with
+      | g_rec G => gunrollings n (g_open 0 (g_rec G) G)
+      | _ => G
+      end
+    | 0 => G
+    end.
+
+  Definition gunroll G := gunrollings (depth_gty G) G.
+
+  Lemma gunroll_not_rec G G': gunroll G != g_rec G'.
+  *)
+
+  Lemma ic_proj r :
+    forall iG iL cG cL,
+    g_closed iG ->
+    project iG r == Some iL ->
+    GUnroll iG cG ->
+    LUnroll iL cL ->
+    Project r cG cL.
+  Proof.
+    cofix CIh; case=>[|v|G|]/=.
+    - case=>// cG cL _ _ GU.
+      case Eq: _ _ / GU =>//; move => {Eq} LU.
+      case Eq: _ _ / LU =>//; move => {Eq}.
+      by constructor.
+    - case=>// v' cG cL _ _ GU.
+      by case Eq: _ _ / GU.
+    - case Gr: (project G r) => [L|//]; move: Gr=>/eqP-Gr.
+      move=> iL cG cL clG; case: ifP=>[//|L_not_var /eqP-[<-] GU LU].
+      move=>Eq; move: Eq Gr=>/eqP-> Gr /eqP-[<-]{L iL}.
+      case EqG: _ _ /GU=>[//|G'' {cG}cG GU|//]; move: EqG GU=>[<-] GU {G''}.
+      case EqL: _ _ /LU=>[//|L'' {cL}cL LU|//]; move: EqL LU=>[<-] LU {L''}.
+      move: Gr => /project_closed /(_ clG L_not_var)/eqP-Gr.
+      case: cG GU => [GU|].
+      case Eq: rg_end /GU =>[|G'' cG' GU|]//.
+      admit.
+      case: cL LU => [LU|].
+      move: clG => /gopen_closed-clG.
+      move: clG Gr LU GU.
+
+      elim/gty_ind1: G L Gr GU L_not_var LU.
+      * admit.
+      * admit.
+      case EqG: _ _ /GU=>[//|G'' {cG}cG GU|//]; move: EqG GU=>[<-] GU {G''}.
+      case EqL: _ _ /LU=>[//|L'' {cL}cL LU|//]; move: EqL LU=>[<-] LU {L''}.
+      admit.
+      apply: CIh.
+
+  (*
+  CoFixpoint project2 (g : rg_ty) (r : role) : option rl_ty :=
+   *)
+
+End CProject.
+
+(*
   Fixpoint project2 (g : rg_ty) (r : role) : option l_ty :=
     match g with
     | g_end => Some l_end
@@ -243,28 +786,6 @@ Section Project.
       + by apply: (Ih K)=>//; right.
   Qed.
 
-  Definition full_project G p q :=
-    match project G p with
-    | Some L => partial_proj L q
-    | None => None
-    end.
-
-  Definition fullproj_all Ks p q :=
-    match prj_all Ks p with
-    | Some LKs => pprj_all LKs q
-    | None => None
-    end.
-
-  Lemma fullproject_some p q G L S
-    : project G p == Some L -> partial_proj L q == Some S ->
-      full_project G p q = Some S.
-  Proof. by rewrite /full_project =>/eqP-> /eqP. Qed.
-
-  Lemma def_fprojall p q G L S
-    : prj_all G p == Some L -> pprj_all L q == Some S ->
-      fullproj_all G p q = Some S.
-  Proof. by rewrite /fullproj_all =>/eqP-> /eqP. Qed.
-
   Lemma option_comm A B C (x : option A) (f : A -> option B) (g : B -> C) z z' :
     match
       match x with
@@ -296,56 +817,6 @@ Section Project.
     by case: ifP.
   Qed.
 
-  Lemma fprojall_eq Ks p q Ks0 Ks1
-    : (forall K, member K Ks ->
-                 forall S S', full_project K.cnt p q == Some S ->
-                              full_project K.cnt q p == Some S' ->
-                              S' = dual S) ->
-      fullproj_all Ks p q == Some Ks0 ->
-      fullproj_all Ks q p == Some Ks1 ->
-      Ks1 = [seq (x.lbl, (x.mty, dual x.cnt)) | x <- Ks0].
-  Proof.
-    elim: Ks =>[|K Ks Ih] /= in Ks0 Ks1 *.
-    - by move=> H; rewrite /fullproj_all/==>/eqP-[<-]/eqP-[<-].
-    - move=> H; rewrite /fullproj_all/=.
-      case Kp: (project K.cnt p)=>[Lp|]//; case Ksp: (prj_all Ks p)=>[Lsp|]//=.
-      case Ep: (partial_proj Lp q)=>[Sp|]//; case Esp: (pprj_all Lsp q)=>[Ssp|]//=.
-      case Kq: (project K.cnt q)=>[Lq|]//; case Ksq: (prj_all Ks q)=>[Lsq|]//=.
-      case Eq: (partial_proj Lq p)=>[Sq|]//; case Esq: (pprj_all Lsq p)=>[Ssq|]//=.
-      move=>/eqP-[<-]/eqP-[<-]/=.
-      rewrite -(H K _ Sp Sq) /full_project ?Kp ?Ep ?Kq ?Eq //; last (by left).
-      congr cons; apply/Ih; rewrite /fullproj_all ?Ksp ?Esp ?Ksq ?Esq//.
-      by move=> K0 K0Ks; apply/H; right.
-  Qed.
-
-  Lemma merge_some (A : eqType)
-        (K : lbl * (mty * A))
-        (Ks : seq (lbl * (mty * A))) L
-    : merge K.cnt [seq K0.cnt | K0 <- Ks] == Some L -> K.cnt = L.
-  Proof. by elim: Ks=>[/eqP-[]//|K' Ks Ih/=]; case:ifP. Qed.
-
-  Lemma merge_pprj L' Ks L p S
-    : merge L' [seq K.cnt | K <- Ks] == Some L -> partial_proj L p == Some S ->
-      exists Ks', pprj_all Ks p = Some Ks' /\
-                  merge S [seq K.cnt | K <- Ks'] = Some S.
-  Proof.
-    elim: Ks=>[_|K' Ks Ih]/=; first (by exists [::]; split); move: Ih.
-    case: ifP=>///eqP<- Ih M_L'; move: (merge_some M_L')=>-> /eqP-L_S.
-    rewrite L_S; move: L_S=>/eqP-L_S; move: (Ih M_L' L_S) => [Ks' [Ksp M_S]].
-    by exists ((K'.lbl, (K'.mty, S)):: Ks'); rewrite Ksp /= eq_refl M_S.
-  Qed.
-
-  Lemma mergeall_pprj Ks L p S
-    : merge_all [seq K.cnt | K <- Ks] == Some L -> partial_proj L p == Some S ->
-      exists Ks', pprj_all Ks p = Some Ks' /\
-                  merge_all [seq K.cnt | K <- Ks'] = Some S.
-  Proof.
-    case: Ks=>[//|K Ks]/=; move=> H; move: (merge_some H)=>KL.
-    move: KL H=>-> H /eqP-L_S; rewrite L_S; move: L_S=>/eqP-L_S.
-    move: (merge_pprj H L_S)=>[Ks' [Ksp M_S]].
-    by exists ((K.lbl, (K.mty, S)) :: Ks'); rewrite Ksp/= M_S.
-  Qed.
-
   Lemma mergeall_merge (A : eqType) S (Ks : seq (lbl * (mty * A)))
     : merge_all [seq K.cnt | K <- Ks] == Some S ->
       merge S [seq K.cnt | K <- Ks] == Some S.
@@ -353,125 +824,6 @@ Section Project.
     case: Ks=>[| K Ks /= H]//=.
     move: (merge_some H)=>/eqP; case: ifP=>///eqP-K_S.
     by move: K_S H=>->.
-  Qed.
-
-  Lemma fun_mergeall (A B : eqType) (f : A -> B) (Ks : seq (lbl * (mty * A))) X
-    : injective f ->
-      merge_all [seq f x.cnt | x <- Ks] == Some (f X) ->
-      merge_all [seq x.cnt | x <- Ks] == Some X.
-  Proof.
-    case: Ks=>[//|K Ks/=] I; elim: Ks=>[|K' Ks]//=.
-    - by move=>/eqP-[/I->].
-    - by move=> Ih; case: ifP=>///eqP-[/I->]; rewrite eq_refl=>/Ih.
-  Qed.
-
-  Lemma dualproj_msg Ks p q Ks0 Ks1 S S' a1 a2 :
-    (forall s s0 : seq (lbl * (mty * s_ty)),
-        fullproj_all Ks p q == Some s ->
-        fullproj_all Ks q p == Some s0 ->
-        s0 = [seq (x.lbl, (x.mty, dual x.cnt)) | x <- s]) ->
-    a2 == dual_act a1 ->
-    prj_all Ks p = Some Ks0 ->
-    prj_all Ks q = Some Ks1 ->
-    partial_proj (l_msg a1 q Ks0) q == Some S ->
-    partial_proj (l_msg a2 p Ks1) p == Some S' ->
-    S' = dual S.
-  Proof.
-    move=> Ih /eqP-a12 Lp Lq; rewrite !partialproj_all !eq_refl.
-    case Kspq: (pprj_all Ks0) => [Ks0'|//].
-    case Ksqp: (pprj_all Ks1) => [Ks1'|//].
-    move=> /eqP-[<-]/eqP-[<-]/=; congr s_msg=>//.
-    by rewrite (Ih Ks0' Ks1') /fullproj_all ?Lp ?Kspq ?Lq ?Ksqp.
-  Qed.
-
-  Lemma dualproj_all Ks p q Ks0 Ks1 S S' s a :
-    (forall s s0 : seq (lbl * (mty * s_ty)),
-        fullproj_all Ks p q == Some s ->
-        fullproj_all Ks q p == Some s0 ->
-        s0 = [seq (x.lbl, (x.mty, dual x.cnt)) | x <- s]) ->
-    prj_all Ks p = Some Ks0 ->
-    prj_all Ks q = Some Ks1 ->
-    (s == q) = false ->
-    partial_proj (l_msg a s Ks0) q == Some S ->
-    match merge_all [seq K.cnt | K <- Ks1] with
-    | Some L => partial_proj L p
-    | None => None
-    end == Some S' ->
-    S' = dual S.
-  Proof.
-    move=> Ih Ksp Ksq s_neq_q; rewrite !partialproj_all s_neq_q.
-    case Kspq: (pprj_all Ks0) => [Ks0'|//]; move => EqS.
-    case Ksqp: (merge_all [seq K.cnt | K <- Ks1]) => [L'|//].
-    move: Ksqp=>/eqP-Ksqp  L'S'.
-    move: (mergeall_pprj Ksqp L'S')=>[Ks' [/eqP-Ks1p /eqP-H]]; move: H EqS.
-    rewrite (Ih Ks0' Ks' ) /fullproj_all ?Ksp ?Kspq ?Ksq//.
-    rewrite -map_comp /comp/= -{1}(dualK S').
-    by move=>/(fun_mergeall dualI)/eqP-> /eqP-[<-]; rewrite dualK.
-  Qed.
-
-  Lemma dualproj_all2 Ks p q Ks0 Ks1 S S' s a :
-    (forall s s0 : seq (lbl * (mty * s_ty)),
-        fullproj_all Ks p q == Some s ->
-        fullproj_all Ks q p == Some s0 ->
-        s0 = [seq (x.lbl, (x.mty, dual x.cnt)) | x <- s]) ->
-    prj_all Ks p = Some Ks0 ->
-    prj_all Ks q = Some Ks1 ->
-    (s == p) = false ->
-    match merge_all [seq K.cnt | K <- Ks0] with
-    | Some L => partial_proj L q
-    | None => None
-    end == Some S ->
-    partial_proj (l_msg a s Ks1) p == Some S' ->
-    S' = dual S.
-  Proof.
-    move=> Ih Ksp Ksq s_neq_q; rewrite !partialproj_all s_neq_q.
-    case Kspq: (pprj_all Ks1) => [Ks0'|//].
-    case Ksqp: (merge_all [seq K.cnt | K <- Ks0]) => [L'|//].
-    move: Ksqp=>/eqP-Ksqp  L'S'.
-    move: (mergeall_pprj Ksqp L'S')=>[Ks' [/eqP-Ks1p /eqP-H]]; move: H.
-    rewrite (Ih Ks' Ks0' ) /fullproj_all ?Ksp ?Ksq ?Kspq//.
-    rewrite -map_comp /comp/= -{1}(dualK S').
-    move=>H1 /(fun_mergeall dualI)/eqP-H2; move: H2 H1.
-    by move=>->/eqP-[<-]; rewrite dualK.
-  Qed.
-
-  Lemma all_compat G S S' p q :
-    p != q ->
-    full_project G p q == Some S ->
-    full_project G q p == Some S' ->
-    S' = dual S.
-  Proof.
-    move=>/negPf-p_neq_q.
-    elim/gty_ind1: G => [|v|G Ih| a r s Ks Ih] in S S' *.
-    - by do ! (move=>/eqP-[<-]).
-    - by do ! (move=>/eqP-[<-]).
-    - rewrite /full_project/=.
-      case Ep: (project G p)=>[Lp|//]; case Eq: (project G q)=>[Lq|//].
-      do ! case: ifP=>[//|_]/=.
-      case Epq: (partial_proj Lp q)=>[Spq|//].
-      case Eqp: (partial_proj Lq p)=>[Sqp|//].
-      move: Eq =>/eqP/fullproject_some-H0; move: Eqp=>/eqP/H0/eqP/Ih-{H0 Ih}Ih.
-      move: Ep =>/eqP/fullproject_some-H0; move: Epq=>/eqP/H0/eqP/Ih{H0 Ih}->.
-      case: ifP=>[/eqP->/eqP-[<-]/eqP-[<-]//|].
-      by rewrite -{1}(dualK Spq); case: ifP=>[/eqP->//|_ _ /eqP-[<-] /eqP-[<-]].
-    - move: Ih=>/fprojall_eq-Ih; rewrite /full_project !project_msg.
-      case Ksp: (prj_all Ks) => [Ks0|//]; case Ksq: (prj_all Ks) => [Ks1|//].
-      case: ifP=>// -r_neq_s.
-      do ! (case: ifP=>[/eqP->|]//; rewrite ?p_neq_q ?r_neq_s //).
-      * by apply: (dualproj_msg Ih).
-      * by apply: (dualproj_all Ih).
-      * by move=> _; apply: (dualproj_msg Ih).
-      * by move=> r_neq_q _; apply: (dualproj_all Ih).
-      * by move=> s_neq_p _; apply: (dualproj_all2 Ih).
-      * by move=> _ _ r_neq_p; apply: (dualproj_all2 Ih).
-      * case M_Ks0: (merge_all [seq K.cnt | K <- Ks0]) => [L'|//].
-        case M_Ks1: (merge_all [seq K.cnt | K <- Ks1]) => [L|//].
-        move: M_Ks0 M_Ks1 =>/eqP-M_Ks0 /eqP-M_Ks1 _ _ _ _ L'S LS'.
-        move: (mergeall_pprj M_Ks0 L'S)=>[Ks' [/eqP-Ks0q /eqP-H]]; move: H.
-        move: (mergeall_pprj M_Ks1 LS')=>[Ks'' [/eqP-Ks1p /eqP-H]]; move: H.
-        rewrite (Ih Ks' Ks'') /fullproj_all ?Ksp ?Ksq // -map_comp/comp/=.
-        rewrite -{1}(dualK S'); move=>/(fun_mergeall dualI)/eqP->/eqP-[<-].
-        by rewrite dualK.
   Qed.
 
   Fixpoint proj_ps (G : rg_ty) (ps : seq role) :=
@@ -496,6 +848,9 @@ Section Project.
     | _, _ => None
     end%fmap.
 
+  Close Scope mpst_scope.
+
+
   Lemma proj_send p q KsG E :
     proj_env (g_msg None p q KsG) == Some E ->
     exists KsL, (prj_all2 KsG p == Some KsL)
@@ -507,7 +862,4 @@ Section Project.
     (prj_all2 Ks p == Some KsL) ->
     exists L, (project2 Gp p == Some L) && (lookup lb KsL == Some (t, L)).
   Admitted.
-
-  Close Scope mpst_scope.
-
-End Project.
+*)
